refactor more for binary search

examples/binary_search.v
@@ -5,128 +5,253 @@ Require Import isla.adequacy.
 Require Import isla.examples.sys_regs.
 From isla.instructions.binary_search Require Import instrs.
 
-Definition args_registers : list string :=
-  ["R0"; "R1"; "R2"; "R3"; "R4"; "R5"; "R6"; "R7"].
+Global Instance valu_inhabited : Inhabited valu := populate (Val_Bool true).
+Definition bool_to_bv (n : N) (b : bool) : bv n :=
+  Z_to_bv n (Z_of_bool b).
+
+Lemma bv_extract_bool_to_bv n1 n2 b:
+  bv_extract 0 n1 (bool_to_bv n2 b) = bool_to_bv n1 b.
+Proof.
+  apply bv_eq.
+  rewrite bv_extract_unsigned.
+Admitted.
+Lemma bv_not_bool_to_bv b:
+  bv_not (bool_to_bv 1 b) = bool_to_bv 1 (negb b).
+Proof. apply bv_eq. by destruct b. Qed.
+
+
+Section proof.
+Context `{!islaG Σ} `{!threadG}.
+
 Definition tmp_registers : list string :=
   ["R9"; "R10"; "R11"; "R12"; "R13"; "R14"; "R15"; "R16"; "R17"].
 
-
-Definition c_call `{!islaG Σ} `{!threadG} (args : list (bv 64)) (P : iProp Σ) (Q : list (bv 64) → iProp Σ) : iProp Σ :=
-  ∃ (ret : bv 64),
-  ∃ (sp r8 r19 r20 r21 r22 r23 r24 r25 r26 r27 r28 r29 : bv 64),
+Definition c_call (P : list valu → ((list valu → iProp Σ) → iProp Σ) → iProp Σ) : iProp Σ :=
+  ∃ (sp ret : bv 64),
   reg_col sys_regs ∗
   reg_col CNVZ_regs ∗
   reg_col ((λ r, (RegColDirect r, None)) <$> tmp_registers) ∗
-  ([∗ list] r;a∈args_registers;args, r ↦ᵣ Val_Bits (a : bv 64)) ∗
-  "R8" ↦ᵣ Val_Bits r8 ∗
-  "R19" ↦ᵣ Val_Bits r19 ∗
-  "R20" ↦ᵣ Val_Bits r20 ∗
-  "R21" ↦ᵣ Val_Bits r21 ∗
-  "R22" ↦ᵣ Val_Bits r22 ∗
-  "R23" ↦ᵣ Val_Bits r23 ∗
-  "R24" ↦ᵣ Val_Bits r24 ∗
-  "R25" ↦ᵣ Val_Bits r25 ∗
-  "R26" ↦ᵣ Val_Bits r26 ∗
-  "R27" ↦ᵣ Val_Bits r27 ∗
-  "R28" ↦ᵣ Val_Bits r28 ∗
-  "R29" ↦ᵣ Val_Bits r29 ∗
+  "R0" ↦ᵣ: λ r0,
+  "R1" ↦ᵣ: λ r1,
+  "R2" ↦ᵣ: λ r2,
+  "R3" ↦ᵣ: λ r3,
+  "R4" ↦ᵣ: λ r4,
+  "R5" ↦ᵣ: λ r5,
+  "R6" ↦ᵣ: λ r6,
+  "R7" ↦ᵣ: λ r7,
+  "R8" ↦ᵣ: λ r8,
+  "R19" ↦ᵣ: λ r19,
+  "R20" ↦ᵣ: λ r20,
+  "R21" ↦ᵣ: λ r21,
+  "R22" ↦ᵣ: λ r22,
+  "R23" ↦ᵣ: λ r23,
+  "R24" ↦ᵣ: λ r24,
+  "R25" ↦ᵣ: λ r25,
+  "R26" ↦ᵣ: λ r26,
+  "R27" ↦ᵣ: λ r27,
+  "R28" ↦ᵣ: λ r28,
+  "R29" ↦ᵣ: λ r29,
   "R30" ↦ᵣ Val_Bits ret ∗
   "SP_EL2" ↦ᵣ Val_Bits sp ∗
-  P ∗
+  P [r0; r1; r2; r3; r4; r5; r6; r7] (λ Q,
   instr_pre (bv_unsigned ret) (
-    ∃ (r0 r1 r2 r3 r4 r5 r6 r7 r8 : bv 64),
       reg_col sys_regs ∗
       reg_col CNVZ_regs ∗
-      "R0" ↦ᵣ Val_Bits r0 ∗
-      "R1" ↦ᵣ Val_Bits r1 ∗
-      "R2" ↦ᵣ Val_Bits r2 ∗
-      "R3" ↦ᵣ Val_Bits r3 ∗
-      "R4" ↦ᵣ Val_Bits r4 ∗
-      "R5" ↦ᵣ Val_Bits r5 ∗
-      "R6" ↦ᵣ Val_Bits r6 ∗
-      "R7" ↦ᵣ Val_Bits r7 ∗
-      "R8" ↦ᵣ Val_Bits r8 ∗
+      reg_col ((λ r, (RegColDirect r, None)) <$> ["R0"; "R1"; "R2"; "R3"; "R4"; "R5"; "R6"; "R7"]) ∗
       reg_col ((λ r, (RegColDirect r, None)) <$> tmp_registers) ∗
-      "R19" ↦ᵣ Val_Bits r19 ∗
-      "R20" ↦ᵣ Val_Bits r20 ∗
-      "R21" ↦ᵣ Val_Bits r21 ∗
-      "R22" ↦ᵣ Val_Bits r22 ∗
-      "R23" ↦ᵣ Val_Bits r23 ∗
-      "R24" ↦ᵣ Val_Bits r24 ∗
-      "R25" ↦ᵣ Val_Bits r25 ∗
-      "R26" ↦ᵣ Val_Bits r26 ∗
-      "R27" ↦ᵣ Val_Bits r27 ∗
-      "R28" ↦ᵣ Val_Bits r28 ∗
-      "R29" ↦ᵣ Val_Bits r29 ∗
+      "R0" ↦ᵣ: λ r0',
+      "R1" ↦ᵣ: λ r1',
+      "R2" ↦ᵣ: λ r2',
+      "R3" ↦ᵣ: λ r3',
+      "R4" ↦ᵣ: λ r4',
+      "R5" ↦ᵣ: λ r5',
+      "R6" ↦ᵣ: λ r6',
+      "R7" ↦ᵣ: λ r7',
+      "R8" ↦ᵣ: λ r8',
+      "R19" ↦ᵣ r19 ∗
+      "R20" ↦ᵣ r20 ∗
+      "R21" ↦ᵣ r21 ∗
+      "R22" ↦ᵣ r22 ∗
+      "R23" ↦ᵣ r23 ∗
+      "R24" ↦ᵣ r24 ∗
+      "R25" ↦ᵣ r25 ∗
+      "R26" ↦ᵣ r26 ∗
+      "R27" ↦ᵣ r27 ∗
+      "R28" ↦ᵣ r28 ∗
+      "R29" ↦ᵣ r29 ∗
       "R30" ↦ᵣ Val_Bits ret ∗
       "SP_EL2" ↦ᵣ Val_Bits sp ∗
-      Q [r0; r1; r2; r3; r4; r5; r6; r7; r8] ∗
-      True
+      Q [r0'; r1'; r2'; r3'; r4'; r5'; r6'; r7'; r8']
+  )).
+Hint Unfold c_call : isla_unfold.
+
+Definition comp_spec : iProp Σ :=
+  (c_call (λ args R, R (λ rets, ∃ b : bool, ⌜rets !!! 0%nat = Val_Bits (bool_to_bv 64 b)⌝)))%I.
+Hint Unfold comp_spec : isla_unfold.
+
+Definition a40_tst_imm_spec : iProp Σ :=
+  ∃ (v : bv 64),
+  reg_col CNVZ_regs ∗
+  "R0" ↦ᵣ Val_Bits v ∗
+  instr_pre 0x0000000010300044 (
+    "R0" ↦ᵣ Val_Bits v ∗
+    "PSTATE" # "N" ↦ᵣ Val_Bits [BV{1} 0] ∗
+    "PSTATE" # "Z" ↦ᵣ Val_Bits (bv_not (bv_extract 0 1 v)) ∗
+    "PSTATE" # "C" ↦ᵣ Val_Bits [BV{1} 0] ∗
+    "PSTATE" # "V" ↦ᵣ Val_Bits [BV{1} 0] ∗
+    True
   ).
+Hint Unfold a40_tst_imm_spec : isla_unfold.
 
-Arguments c_call _ _ _ /.
+Lemma a40_has_tst_imm_spec :
+  instr 0x0000000010300040 (Some a40) -∗
+  instr_body 0x0000000010300040 (a40_tst_imm_spec).
+Proof.
+  iStartProof. rewrite /a40_tst_imm_spec.
+  repeat liAStep; liShow.
+  Unshelve. all: prepare_sidecond.
+  all: try bv_solve.
+  - bv_simplify.
+    rewrite Z.shiftr_eq_0 // ?Z.land_nonneg; [lia|].
+    apply: Z.le_lt_trans; [apply Z.log2_land; bv_solve| bv_solve].
+  - admit.
+  - bv_simplify.
+    rewrite Z.shiftr_eq_0 // ?Z.land_nonneg; [lia|].
+    apply: Z.le_lt_trans; [apply Z.log2_land; bv_solve| bv_solve].
+  - admit.
+Admitted.
 
-Definition comp_spec `{!islaG Σ} `{!threadG} : iProp Σ :=
-  ∃ r0 r1 r2 r3 r4 r5 r6 r7,
-  c_call [r0; r1; r2; r3; r4; r5; r6; r7] True (λ rets, True).
+Definition a44_csel_spec : iProp Σ :=
+  ∃ (v1 v2 : bv 64) (pstaten pstatez pstatec pstatev : bv 1),
+  "PSTATE" # "N" ↦ᵣ Val_Bits pstaten ∗
+  "PSTATE" # "Z" ↦ᵣ Val_Bits pstatez ∗
+  "PSTATE" # "C" ↦ᵣ Val_Bits pstatec ∗
+  "PSTATE" # "V" ↦ᵣ Val_Bits pstatev ∗
+  "R20" ↦ᵣ Val_Bits v1 ∗
+  "R24" ↦ᵣ Val_Bits v2 ∗
+  instr_pre 0x0000000010300048 (
+    "R20" ↦ᵣ Val_Bits (ite (bool_decide (bv_unsigned pstatez = 0)) v1 v2) ∗
+    "R24" ↦ᵣ Val_Bits v2 ∗
+    "PSTATE" # "N" ↦ᵣ Val_Bits pstaten ∗
+    "PSTATE" # "Z" ↦ᵣ Val_Bits pstatez ∗
+    "PSTATE" # "C" ↦ᵣ Val_Bits pstatec ∗
+    "PSTATE" # "V" ↦ᵣ Val_Bits pstatev ∗
+    True
+  ).
+Hint Unfold a44_csel_spec : isla_unfold.
+
+Lemma a44_has_csel_spec :
+  instr 0x0000000010300044 (Some a44) -∗
+  instr_body 0x0000000010300044 (a44_csel_spec).
+Proof.
+  iStartProof. rewrite /a44_csel_spec.
+  repeat liAStep; liShow.
+  Unshelve. all: prepare_sidecond.
+  all: try bv_solve.
+  - rewrite bool_decide_true //.
+    admit.
+Admitted.
+
+Definition a48_csinc_spec : iProp Σ :=
+  ∃ (v1 v2 : bv 64) (pstaten pstatez pstatec pstatev : bv 1),
+  "PSTATE" # "N" ↦ᵣ Val_Bits pstaten ∗
+  "PSTATE" # "Z" ↦ᵣ Val_Bits pstatez ∗
+  "PSTATE" # "C" ↦ᵣ Val_Bits pstatec ∗
+  "PSTATE" # "V" ↦ᵣ Val_Bits pstatev ∗
+  "R23" ↦ᵣ Val_Bits v1 ∗
+  "R24" ↦ᵣ Val_Bits v2 ∗
+  instr_pre 0x000000001030004c (
+    "R23" ↦ᵣ Val_Bits (ite (bool_decide (bv_unsigned pstatez = 1)) v1 (bv_add_Z v2 1)) ∗
+    "R24" ↦ᵣ Val_Bits v2 ∗
+    "PSTATE" # "N" ↦ᵣ Val_Bits pstaten ∗
+    "PSTATE" # "Z" ↦ᵣ Val_Bits pstatez ∗
+    "PSTATE" # "C" ↦ᵣ Val_Bits pstatec ∗
+    "PSTATE" # "V" ↦ᵣ Val_Bits pstatev ∗
+    True
+  ).
+Hint Unfold a48_csinc_spec : isla_unfold.
+
+Lemma a48_has_csinc_spec :
+  instr 0x0000000010300048 (Some a48) -∗
+  instr_body 0x0000000010300048 (a48_csinc_spec).
+Proof.
+  iStartProof. rewrite /a48_csinc_spec.
+  repeat liAStep; liShow.
+  Unshelve. all: prepare_sidecond.
+  all: try bv_solve.
+  - rewrite bool_decide_false //=.
+    rename select (_ ≠ _) into Hz. contradict Hz. bv_solve.
+Qed.
 
 
-Definition binary_search_loop_spec `{!islaG Σ} `{!threadG} : iProp Σ :=
-  ∃ (x l r comp xs tmp2 tmp5 : bv 64) (data : list (bv 64)),
+Definition binary_search_loop_spec : iProp Σ :=
+  ∃ (x l r comp xs tmp2 sp : bv 64) (data : list (bv 64)),
   reg_col sys_regs ∗
   reg_col CNVZ_regs ∗
-  reg_col ((λ r, (RegColDirect r, None)) <$> ["R0"; "R1"; "R2"; "R3"; "R4"; "R5"; "R6"; "R7"; "R8"; "R9"; "R10"; "R11"; "R12"; "R13"; "R14"; "R15"; "R16"; "R17" ]) ∗
+  reg_col ((λ r, (RegColDirect r, None)) <$> ["R0"; "R1"; "R2"; "R3"; "R4"; "R5"; "R6"; "R7"; "R8"; "R9"; "R10"; "R11"; "R12"; "R13"; "R14"; "R15"; "R16"; "R17"; "R25"; "R26"; "R27"; "R28"; "R29"; "R30" ]) ∗
   "R19" ↦ᵣ Val_Bits x ∗
   "R20" ↦ᵣ Val_Bits r ∗
   "R21" ↦ᵣ Val_Bits xs ∗
   "R22" ↦ᵣ Val_Bits comp ∗
   "R23" ↦ᵣ Val_Bits l ∗
   "R24" ↦ᵣ Val_Bits tmp2 ∗
-  "R30" ↦ᵣ Val_Bits tmp5 ∗
+  "SP_EL2" ↦ᵣ Val_Bits sp ∗
   xs ↦ₘ∗ data ∗
   ⌜bv_unsigned l < bv_unsigned r ≤ length data⌝ ∗
   ⌜bv_unsigned xs + (length data) * 8 < 2 ^ 52⌝ ∗
   □ instr_pre (bv_unsigned comp) comp_spec ∗
   instr_pre 0x0000000010300054 (
-    ∃ (tmp2 tmp5 : bv 64),
+    ∃ (l' r' tmp2 : bv 64),
       reg_col sys_regs ∗
       reg_col CNVZ_regs ∗
-      reg_col ((λ r, (RegColDirect r, None)) <$> ["R0"; "R1"; "R2"; "R3"; "R4"; "R5"; "R6"; "R7"; "R8"; "R9"; "R10"; "R11"; "R12"; "R13"; "R14"; "R15"; "R16"; "R17" ]) ∗
+      reg_col ((λ r, (RegColDirect r, None)) <$> ["R0"; "R1"; "R2"; "R3"; "R4"; "R5"; "R6"; "R7"; "R8"; "R9"; "R10"; "R11"; "R12"; "R13"; "R14"; "R15"; "R16"; "R17"; "R25"; "R26"; "R27"; "R28"; "R29"; "R30" ]) ∗
       "R19" ↦ᵣ Val_Bits x ∗
-      "R20" ↦ᵣ Val_Bits r ∗
+      "R20" ↦ᵣ Val_Bits r' ∗
       "R21" ↦ᵣ Val_Bits xs ∗
       "R22" ↦ᵣ Val_Bits comp ∗
-      "R23" ↦ᵣ Val_Bits l ∗
+      "R23" ↦ᵣ Val_Bits l' ∗
       "R24" ↦ᵣ Val_Bits tmp2 ∗
-      "R30" ↦ᵣ Val_Bits tmp5 ∗
+      "SP_EL2" ↦ᵣ Val_Bits sp ∗
       xs ↦ₘ∗ data ∗
       True
   )
 .
+Hint Unfold binary_search_loop_spec : isla_unfold.
 
-Arguments binary_search_loop_spec /.
-
-Lemma binary_search_loop `{!islaG Σ} `{!threadG} :
+Lemma binary_search_loop :
   instr 0x000000001030002c (Some a2c) -∗
   instr 0x0000000010300030 (Some a30) -∗
   instr 0x0000000010300034 (Some a34) -∗
   instr 0x0000000010300038 (Some a38) -∗
   instr 0x000000001030003c (Some a3c) -∗
-  instr 0x0000000010300040 (Some a40) -∗
-  instr 0x0000000010300044 (Some a44) -∗
-  instr 0x0000000010300048 (Some a48) -∗
+  (* instr 0x0000000010300040 (Some a40) -∗ *)
+  instr_body 0x0000000010300040 (a40_tst_imm_spec) -∗
+  (* instr 0x0000000010300044 (Some a44) -∗ *)
+  instr_body 0x0000000010300044 (a44_csel_spec) -∗
+  (* instr 0x0000000010300048 (Some a48) -∗ *)
+  instr_body 0x0000000010300048 (a48_csinc_spec) -∗
   instr 0x000000001030004c (Some a4c) -∗
   instr 0x0000000010300050 (Some a50) -∗
   □ instr_pre 0x000000001030002c binary_search_loop_spec -∗
   instr_body 0x000000001030002c binary_search_loop_spec.
 Proof.
-  iStartProof.
+  iStartProof. rewrite {2}/binary_search_loop_spec.
   Time repeat liAStep; liShow.
   liInst Hevar (Z.to_nat (bv_unsigned l + (bv_unsigned r - bv_unsigned l) `div` 2)).
   Time repeat liAStep; liShow.
-  iEval (rewrite /comp_spec /=).
-  Time repeat liAStep; liShow.
 
+  Unshelve. all: prepare_sidecond.
+  - bv_simplify.
+    autorewrite with bv_unfolded_to_arith.
+    have -> : (bv_wrap 64 (bv_unsigned l) + bv_wrap 64
+                (bv_wrap 64
+                   (bv_wrap 64 (bv_wrap 64 (bv_unsigned r) + bv_wrap 64 (bv_wrap 64 (- bv_unsigned l - 1))) + 1)
+                   `div` 2 ^ 1))
+             = (bv_unsigned l + (bv_unsigned r - bv_unsigned l) `div` 2) by bv_solve.
+    rewrite (bv_wrap_small 61 _); [|bv_solve].
+    bv_solve.
+  - bv_solve.
+  - admit.
 Abort.
 
 Lemma binary_search `{!islaG Σ} `{!threadG} :
@@ -172,3 +297,4 @@ Proof.
   iStartProof.
   Time repeat liAStep; liShow.
 Abort.
+End proof.
